试证明 $\nabla^2\left(\frac{\mathrm e^{-kr}}{r}\right)=k^2\frac{\mathrm e^{-kr}}{r}$ 。式中 $k$ 为常数


$$
\left\{
\begin{align}
\frac {\part \left(\frac{\mathrm e^{-kr}}{r}\right)}{\part r}&=\frac{-e^{-kr}(1+kr)}{r^2}\\[3mm]
\frac{\part r}{\part x}&=\frac{x}{\sqrt{x^2+y^2+z^2}}=\frac{x}{r}
\end{align}
\right.
$$

$$
F_x=\frac{\part \left(\frac{\mathrm e^{-kr}}{\part r}\right)}{r}\frac{\part r}{\part x}=\frac{-e^{-kr}(1+kr)}{r^3}x
$$





$$
\begin{align}
F_{xx} &= \frac{\part F_x}{\part x}=\frac{\part \left(\frac{-e^{-kr}(1+kr)}{r^3}x\right)}{\part x}\\[3mm]
&=\frac{-e^{-kr}(1+kr)}{r^3}+x\frac{\part\left(\frac{-e^{-kr}(1+kr)}{r^3}\right)}{\part r}\frac{\part r}{\part x}\\[3mm]
&=\frac{-e^{-kr}(1+kr)}{r^3}+\left(\frac{r^3\left(-\mathrm e^{-kr}(1+kr)\right)'-3r^2(-\mathrm e^{-kr}(1+kr))}{r^6}\right)\frac{x^2}{r}\\[3mm]
&=\frac{-e^{-kr}(1+kr)}{r^3}+\left(\frac{r^3(k\mathrm e^{-kr}(1+kr)-k\mathrm e^{-kr})-3r^2(-\mathrm e^{-kr}(1+kr))}{r^6}\right)\frac{x^2}{r}\\[3mm]
&=\frac{-e^{-kr}(1+kr)}{r^3}+\left(\frac{k^2r^2\mathrm e^{-kr}+3\mathrm e^{-kr}(1+kr)}{r^4}\right)\frac{x^2}{r}\\[3mm]
&=\frac{-e^{-kr}(1+kr)}{r^3}+\frac{k^2r^2\mathrm e^{-kr}+3\mathrm e^{-kr}(1+kr)}{r^5}x^2\\[3mm]

\end{align}
$$

对 x y z 求偏导得结果类似 (只要将上式的 x 换成 y z 即可)，最后相加得到
$$
\begin{align}
&F_{xx}+F_{yy}+F_{zz}\\[3mm]
&=\frac{-3e^{-kr}(1+kr)}{r^3}+\frac{k^2r^2\mathrm e^{-kr}+3\mathrm e^{-kr}(1+kr)}{r^5}(x^2+y^2+z^2)\\[3mm]
&=\frac{-3e^{-kr}(1+kr)}{r^3}+\frac{k^2r^2\mathrm e^{-kr}+3\mathrm e^{-kr}(1+kr)}{r^3}\\[3mm]
&=k^2\frac{\mathrm e^{-kr}}{r}
\end{align}
$$