$$
f(t)\rightarrow\tau Sa(\frac{\omega \tau}{2})\\
f(t-\frac{\tau}{2})\rightarrow\tau Sa(\frac{\omega \tau}{2})\,\mathrm e^{-j\omega \tau}
$$
$$
\begin{align}
&\qquad\tau Sa(\frac{\omega \tau}{2})\,\mathrm e^{-j\frac{\omega \tau}2}\\[1mm]
&=\frac2\omega \sin(\frac{\omega \tau}{2})\,(\cos(\frac{\omega \tau}2)-j\sin(\frac{\omega\tau}2))\\[1mm]
&=\frac 1 \omega \sin(\omega\tau)-j\frac2\omega \sin^2(\frac{\omega\tau}2)\\[1mm]
&=\frac 1 \omega \sin(\omega\tau)-j\frac1\omega(1-\cos(\omega\tau))\\[1mm]
&=\frac1\omega\sin(\omega\tau)+j\frac1\omega(\cos(\omega\tau)-1)
\end{align}
$$

$$
\begin{align}
&\qquad\int^{\tau}_0\mathrm e^{-j\omega t}\,dt\\[2mm]
&=\frac{1}{-j\omega}\left[\mathrm e^{-j\omega t}\right]^\tau_0\\[2mm]
&=j\frac 1 \omega(\mathrm e^{-j\omega\tau}-1)\\[2mm]
&=j\frac 1 \omega((\cos(\omega\tau)-1)-j\sin(\omega\tau))\\[2mm]
&=\frac1\omega\sin(\omega\tau)+j\frac1\omega(\cos(\omega\tau)-1)
\end{align}
$$

